src/fs/FStar.FunctionalExtensionality.fs
@@ -5,6 +5,3 @@ open Prims
 type ('Aa, 'Ab) efun =
 'Aa  ->  'Ab
 
-
-
-
