Makefile
@@ -4,14 +4,15 @@ FSTAR = $(FSTAR_HOME)/bin/fstar.exe
 FSHARP = fsharpc
 
 FILES = Util.fst Total.fst Par.fst PairHeap.fst AncillaHeap.fst Circuit.fst BoolExp.fst ExprTypes.fst Interpreter.fst
-STDLIB = FStar.FunctionalExtensionality.fst FStar.Set.fst FStar.Heap.fst FStar.ST.fst FStar.All.fst FStar.List.fst FStar.String.fsti
-EX = FStar.Map.fst FStar.IO.fsti FStar.ListProperties.fst
+SUPPORT = FStar.Set FStar.Heap FStar.ST FStar.All FStar.List FStar.String FStar.IO
 
-FSFILES =
+FSFILES = FStar.FunctionalExtensionality.fs # FStar.Heap.fs FStar.ListProperties.fs FStar.Map.fs FStar.Util.fs
 
 FSTSRC = $(addprefix src/, $(FILES))
 FSSRC  = $(addprefix src/fs/, $(STDLIB:.fst=.fs) $(EX:.fst=.fs)  $(FSFILES) $(FILES:.fst=.fs))
 LIB 	 = $(addprefix $(FSTAR_HOME)/lib/, $(STDLIB) $(EX))
+
+EXCL   = $(addprefix --no_extract , $(SUPPORT))
 
 DLLS = $(FSTAR_HOME)/lib/fs/fstarlib.dll $(FSTAR_HOME)/bin/FSharp.PowerPack.dll $(FSTAR_HOME)/bin/FSharp.PowerPack.Compatibility.dll
 FSOPS = $(addprefix -r , $(DLLS))
@@ -20,8 +21,8 @@ verify: $(FSTSRC)
 	$(FSTAR) --z3timeout 60 $^
 
 fs: $(FSTSRC)
-	$(FSTAR) --admit_smt_queries true --codegen FSharp $^
+	$(FSTAR) --admit_smt_queries true --codegen FSharp $(EXCL) $^
 	mv *.fs src/fs/
 
 all: $(FSSRC)
-	$(FSHARP) --mlcompatibility $(FSOPS) -o rever.exe $(FSSRC)
+	$(FSHARP) --mlcompatibility $(FSOPS) -o rever.exe $^
